examples/ProcMemCorrect.v
@@ -1,0 +1,61 @@
+Require Import Bool String List.
+Require Import Lib.CommonTactics Lib.ilist Lib.Word.
+Require Import Lib.Struct Lib.StringBound Lib.FMap Lib.StringEq.
+Require Import Lts.Syntax Lts.Semantics Lts.SemFacts Lts.Equiv Lts.Refinement Lts.Renaming Lts.Wf.
+Require Import Lts.Renaming Lts.Specialize Lts.Tactics Lts.Duplicate.
+
+Require Import Ex.SC Ex.ProcDec Ex.MemCache Ex.L1Cache.
+Require Import Ex.MemCorrect Ex.ProcDecSCN.
+
+Set Implicit Arguments.
+
+Section ProcMem.
+  Variable FifoSize: nat. (* fifo *)
+  Variables RfIdx: nat. (* processor *)
+  Variables IdxBits TagBits LgNumDatas LgDataBytes: nat. (* memory *)
+  Variable Id: Kind.
+
+  Definition AddrSize := L1Cache.AddrBits IdxBits TagBits LgNumDatas LgDataBytes.
+  Hint Unfold AddrSize: MethDefs.
+  
+  Variable dec: DecT 2 AddrSize LgDataBytes RfIdx.
+  Variable execState: ExecStateT 2 AddrSize LgDataBytes RfIdx.
+  Variable execNextPc: ExecNextPcT 2 AddrSize LgDataBytes RfIdx.
+
+  Variable n: nat.
+
+  Definition pdecN := pdecs dec execState execNextPc n.
+  Definition mcache := memCache IdxBits TagBits LgNumDatas LgDataBytes Id FifoSize n. 
+  Definition scN := sc dec execState execNextPc opLd opSt opHt n.
+
+  Theorem pdecN_mcache_refines_scN: (pdecN ++ mcache)%kami <<== scN.
+  Proof.
+    ktrans (pdecN ++ memAtomic AddrSize FifoSize LgDataBytes n)%kami.
+
+    - unfold MethsT; rewrite <-idElementwiseId.
+      apply traceRefines_modular_interacting with (vp:= (@idElementwise _)).
+      + admit.
+      + admit.
+      + admit.
+      + admit.
+      + admit.
+      + admit.
+      + admit.
+      + admit.
+      + admit.
+      + admit.
+      + admit.
+      + admit.
+      + admit.
+      + admit.
+      + auto.
+
+      + krefl.
+      + apply memCache_refines_memAtomic.
+
+    - unfold MethsT; rewrite <-idElementwiseId.
+      apply pdecN_memAtomic_refines_scN.
+  Qed.
+
+End ProcMem.
+
